lib/everparse/3d/EverParse3d.Prelude.fst
@@ -206,19 +206,8 @@ let parse_t_exact n #nz #wk #k #t p
 ////////////////////////////////////////////////////////////////////////////////
 
 inline_for_extraction noextract
-let reader #_ #k #t p = LowParse.PulseParse.Base.reader #t #k (p <: LP.parser k t)
+let reader #_ #k #t p = LowParse.Pulse.ArrayPtr.Int.leaf_reader #t #k (p <: LP.parser k t)
 
-inline_for_extraction noextract
-let read_filter #_ #k #t #p p32 f
-    = LowParse.PulseParse.Combinators.read_filter #k #t p32 f
-
-let squash_of_erased (#a: Type) (x: FStar.Ghost.erased a) : squash a =
-  FStar.Squash.return_squash (FStar.Ghost.reveal x)
-
-let read_impos : reader (parse_impos()) =
-  fun input #pm #v t' f ->
-    let _ = squash_of_erased v in
-    false_elim ()
   
 // ////////////////////////////////////////////////////////////////////////////////
 // // Validators
@@ -265,45 +254,42 @@ let parse_all_zeros = LowParse.Spec.List.parse_list (LowParse.Spec.Combinators.p
 /// UINT8
 let parse____UINT8 = LowParse.Spec.Int.parse_u8
 inline_for_extraction noextract
-let read____UINT8 = LowParse.PulseParse.Base.reader_of_serialized LowParse.Pulse.Int.read_u8
+let read____UINT8 = LowParse.Pulse.ArrayPtr.Int.read_u8 ()
 
 /// UINT8BE
 let parse____UINT8BE = LowParse.Spec.Int.parse_u8
 inline_for_extraction noextract
-let read____UINT8BE = LowParse.PulseParse.Base.reader_of_serialized LowParse.Pulse.Int.read_u8
+let read____UINT8BE = LowParse.Pulse.ArrayPtr.Int.read_u8 ()
 
 /// UInt16BE
 let parse____UINT16BE = LowParse.Spec.Int.parse_u16
 inline_for_extraction noextract
-let read____UINT16BE = LowParse.PulseParse.Base.reader_of_serialized LowParse.Pulse.Int.read_u16
+let read____UINT16BE = LowParse.Pulse.ArrayPtr.Int.read_u16 ()
 
 /// UInt32BE
 let parse____UINT32BE = LowParse.Spec.Int.parse_u32
 inline_for_extraction noextract
-let read____UINT32BE = LowParse.PulseParse.Base.reader_of_serialized LowParse.Pulse.Int.read_u32
+let read____UINT32BE = LowParse.Pulse.ArrayPtr.Int.read_u32 ()
 
 /// UInt64BE
 let parse____UINT64BE = LowParse.Spec.Int.parse_u64
 inline_for_extraction noextract
-let read____UINT64BE = LowParse.PulseParse.Base.reader_of_serialized LowParse.Pulse.Int.read_u64
+let read____UINT64BE = LowParse.Pulse.ArrayPtr.Int.read_u64 ()
 
 
 /// UInt16
 let parse____UINT16 = LowParse.Spec.BoundedInt.parse_u16_le
 inline_for_extraction noextract
-let read____UINT16 = LowParse.PulseParse.Base.reader_of_leaf_reader LowParse.PulseParse.BoundedIntLE.read_u16_le
+let read____UINT16 = LowParse.Pulse.ArrayPtr.IntLE.read_u16_le
 
 /// UInt32
 let parse____UINT32 = LowParse.Spec.BoundedInt.parse_u32_le
 inline_for_extraction noextract
-let read____UINT32 = LowParse.PulseParse.Base.reader_of_leaf_reader LowParse.PulseParse.BoundedIntLE.read_u32_le
+let read____UINT32 = LowParse.Pulse.ArrayPtr.IntLE.read_u32_le
 
 
 /// UInt64
 let parse____UINT64 = LowParse.Spec.Int.parse_u64_le
 inline_for_extraction noextract
-let read____UINT64 = LowParse.PulseParse.Base.reader_of_serialized LowParse.Pulse.Int.read_u64_le
+let read____UINT64 = LowParse.Pulse.ArrayPtr.Int.read_u64_le ()
   
-inline_for_extraction noextract
-let read_unit
-  = LowParse.PulseParse.Combinators.read_ret () (fun _ -> ())
